src/Spec/Modules.v
@@ -2,6 +2,7 @@ Require Import ConcurProc.
 Require Import Equiv.
 Require Import Compile.
 Require Import Abstraction.
+Require Import Helpers.Helpers.
 
 
 (** Combining trace matching with state abstraction. *)
@@ -14,6 +15,7 @@ Section TraceAbs.
   Variable StateLo : Type.
   Variable StateMid : Type.
   Variable absR : StateLo -> StateMid -> Prop.
+  Variable initP : StateLo -> Prop.
 
   Variable lo_step : OpSemantics opLoT StateLo.
   Variable mid_step : OpSemantics opMidT StateMid.
@@ -21,12 +23,13 @@ Section TraceAbs.
   Definition traces_match_abs
                            (ts1 : @threads_state opLoT)
                            (ts2 : @threads_state opMidT) :=
-  forall (sl : StateLo) (sm : StateMid) tr1,
-    exec_prefix lo_step sl ts1 tr1 ->
-    absR sl sm ->
-    exists tr2,
-      exec_prefix mid_step sm ts2 tr2 /\
-      trace_eq tr1 tr2.
+    forall (sl : StateLo) (sm : StateMid) tr1,
+      initP sl ->
+      exec_prefix lo_step sl ts1 tr1 ->
+      absR sl sm ->
+      exists tr2,
+        exec_prefix mid_step sm ts2 tr2 /\
+        trace_eq tr1 tr2.
 
 End TraceAbs.
 
@@ -35,6 +38,7 @@ Module Type Layer.
 
   Axiom opT : Type -> Type.
   Axiom State : Type.
+  Axiom initP : State -> Prop.
   Axiom step : OpSemantics opT State.
 
 End Layer.
@@ -55,10 +59,17 @@ Module Type LayerImpl (l1 : Layer) (l2 : Layer).
     forall ts,
       no_atomics_ts ts ->
       no_atomics_ts (compile_ts ts).
+  Axiom absInitP :
+    forall s1 s2,
+      l1.initP s1 ->
+      absR s1 s2 ->
+      l2.initP s2.
   Axiom compile_traces_match :
     forall ts,
       no_atomics_ts ts ->
-      traces_match_abs absR l1.step l2.step (compile_ts ts) ts.
+      traces_match_abs absR l1.initP l1.step l2.step (compile_ts ts) ts.
+
+  Hint Resolve absInitP.
 
 End LayerImpl.
 
@@ -71,11 +82,18 @@ Module Type LayerImplRequiresRule (l1 : Layer) (l2 : Layer) (r : ProcRule l2).
     forall ts,
       no_atomics_ts ts ->
       no_atomics_ts (compile_ts ts).
+  Axiom absInitP :
+    forall s1 s2,
+      l1.initP s1 ->
+      absR s1 s2 ->
+      l2.initP s2.
   Axiom compile_traces_match :
     forall ts,
       r.follows_protocol ts ->
       no_atomics_ts ts ->
-      traces_match_abs absR l1.step l2.step (compile_ts ts) ts.
+      traces_match_abs absR l1.initP l1.step l2.step (compile_ts ts) ts.
+
+  Hint Resolve absInitP.
 
 End LayerImplRequiresRule.
 
@@ -92,10 +110,17 @@ Module Type LayerImplFollowsRule (l1 : Layer) (l2 : Layer) (r : ProcRule l1).
     forall ts,
       no_atomics_ts ts ->
       r.follows_protocol (compile_ts ts).
+  Axiom absInitP :
+    forall s1 s2,
+      l1.initP s1 ->
+      absR s1 s2 ->
+      l2.initP s2.
   Axiom compile_traces_match :
     forall ts,
       no_atomics_ts ts ->
-      traces_match_abs absR l1.step l2.step (compile_ts ts) ts.
+      traces_match_abs absR l1.initP l1.step l2.step (compile_ts ts) ts.
+
+  Hint Resolve absInitP.
 
 End LayerImplFollowsRule.
 
@@ -123,13 +148,23 @@ Module Link
     eauto.
   Qed.
 
+  Theorem absInitP :
+    forall s1 s2,
+      a.initP s1 ->
+      absR s1 s2 ->
+      c.initP s2.
+  Proof.
+    unfold absR; intros; deex.
+    eauto.
+  Qed.
+
   Theorem compile_traces_match :
     forall ts,
       no_atomics_ts ts ->
-      traces_match_abs absR a.step c.step (compile_ts ts) ts.
+      traces_match_abs absR a.initP a.step c.step (compile_ts ts) ts.
   Proof.
     unfold traces_match_abs; intros.
-    inversion H1; clear H1; intuition idtac.
+    inversion H2; clear H2; intuition idtac.
     edestruct x.compile_traces_match; intuition eauto.
       eapply y.compile_ts_no_atomics; eauto.
     edestruct y.compile_traces_match; intuition eauto.
@@ -161,13 +196,23 @@ Module LinkWithRule
     eauto.
   Qed.
 
+  Theorem absInitP :
+    forall s1 s2,
+      a.initP s1 ->
+      absR s1 s2 ->
+      c.initP s2.
+  Proof.
+    unfold absR; intros; deex.
+    eauto.
+  Qed.
+
   Theorem compile_traces_match :
     forall ts,
       no_atomics_ts ts ->
-      traces_match_abs absR a.step c.step (compile_ts ts) ts.
+      traces_match_abs absR a.initP a.step c.step (compile_ts ts) ts.
   Proof.
     unfold traces_match_abs; intros.
-    inversion H1; clear H1; intuition idtac.
+    inversion H2; clear H2; intuition idtac.
     edestruct x.compile_traces_match; intuition eauto.
       eapply y.compile_ts_follows_protocol; eauto.
       eapply y.compile_ts_no_atomics; eauto.
